Typing.v
@@ -4,6 +4,7 @@ Require Import Types Term.
 Definition env := list typ.
 
 Definition env_fv := foldr (cat \o typ_fv) [::].
+Definition env_bv := foldr (cat \o typ_bv) [::].
 
 Lemma env_fv_intro T x (_ : x \in typ_fv T) :
   forall G, T \in G -> x \in env_fv G.
@@ -14,12 +15,28 @@ Proof.
   - by rewrite orbT.
 Qed.
 
-Definition env_subst s := map (typ_subst s).
-
-Lemma env_subst_typ_fvar G : env_subst typ_fvar G = G.
+Lemma env_bv_intro T x (_ : x \in typ_bv T) :
+  forall G, T \in G -> x \in env_bv G.
 Proof.
-  rewrite /env_subst -(@eq_map _ _ id) ?map_id => // ?.
+  elim => //= ? ? IH.
+  rewrite in_cons mem_cat => /orP [ /eqP <- | /IH -> ].
+  - by rewrite H.
+  - by rewrite orbT.
+Qed.
+
+Definition env_subst s := map (typ_subst s).
+Definition env_open s := map (typ_open s).
+
+Lemma env_subst_fvar G : env_subst typ_fvar G = G.
+Proof.
+  rewrite /env_subst map_id_in // => ? ?.
   by rewrite typ_subst_fvar.
+Qed.
+
+Lemma env_open_bvar G : env_open typ_bvar G = G.
+Proof.
+  rewrite /env_open map_id_in // => ? ?.
+  by rewrite typ_open_bvar.
 Qed.
 
 Lemma env_subst_ext s s' G
@@ -29,13 +46,45 @@ Proof.
   apply /eq_in_map => ? ?.
   apply /typ_subst_ext => ? ?.
   apply /Hext /env_fv_intro; eauto.
-Qed. 
+Qed.
 
-Lemma env_subst_typ_comp s s' G :
+Lemma env_open_ext s s' G
+  (Hext : { in env_bv G, s =1 s' }) :
+  env_open s G = env_open s' G.
+Proof.
+  apply /eq_in_map => ? ?.
+  apply /typ_open_ext => ? ?.
+  apply /Hext /env_bv_intro; eauto.
+Qed.
+
+Corollary env_subst_fvar_eq s G :
+  { in env_fv G, s =1 typ_fvar } ->
+  env_subst s G = G.
+Proof.
+  move => /env_subst_ext ->.
+  exact /env_subst_fvar.
+Qed.
+
+Corollary env_open_bvar_eq s G :
+  { in env_bv G, s =1 typ_bvar } ->
+  env_open s G = G.
+Proof.
+  move => /env_open_ext ->.
+  exact /env_open_bvar.
+Qed.
+
+Lemma env_subst_comp s s' G :
   env_subst s (env_subst s' G) = env_subst (typ_subst s \o s') G.
 Proof.
   rewrite /env_subst -map_comp.
   exact /eq_map /typ_subst_comp.
+Qed.
+
+Lemma env_open_comp s s' G :
+  env_open s (env_open s' G) = env_open (typ_open s \o s') G.
+Proof.
+  rewrite /env_open -map_comp.
+  exact /eq_map /typ_open_comp.
 Qed.
 
 Lemma env_fv_subst s x : forall G,
@@ -47,167 +96,391 @@ Proof.
   exists y; rewrite mem_cat Hin ?orbT; eauto.
 Qed.
 
+Lemma env_fv_subst_intro s x y : forall G,
+  y \in env_fv G ->
+  x \in typ_fv (s y) ->
+  x \in env_fv (env_subst s G).
+Proof.
+  elim => //= ? ? IH.
+  rewrite !mem_cat => /orP [ ] Hin => [ /(typ_fv_subst_intro _ _ _ _ Hin) | /(IH Hin) ] -> //.
+  by rewrite orbT.
+Qed.
+
+Lemma env_bv_open s x : forall G,
+  x \in env_bv (env_open s G) ->
+  exists y, x \in typ_bv (s y) /\ y \in env_bv G.
+Proof.
+  elim => //= ? ? IH.
+  rewrite mem_cat => /orP [ /typ_bv_open | /IH ] [ y [ ? Hin ] ];
+  exists y; rewrite mem_cat Hin ?orbT; eauto.
+Qed.
+
 Inductive typed : env -> trm -> typ -> Prop :=
-  | typed_var G x T :
+  | typed_var G x s T :
       (forall d, nth d G x = T) ->
-      typed G (trm_var x) T
+      (forall x, typ_bv (s x) = [::]) ->
+      typed G (trm_var x) (typ_open s T)
   | typed_abs G t T1 T2 :
+      typ_bv T1 = [::] ->
       typed (T1 :: G) t T2 ->
       typed G (trm_abs t) (typ_arrow T1 T2)
   | typed_app G t1 t2 T1 T2 :
       typed G t1 (typ_arrow T1 T2) ->
       typed G t2 T1 ->
       typed G (trm_app t1 t2) T2
-  | typed_let G t1 t2 T1 T2 :
-      typed G t1 T1 ->
+  | typed_let (L : seq nat) G t1 t2 T1 T2 :
+      (forall s, (forall x, exists y, s x = typ_fvar y /\ y \notin L) -> typed G t1 (typ_open s T1)) ->
       typed (T1 :: G) t2 T2 ->
       typed G (trm_let t1 t2) T2.
 Hint Constructors typed.
 
-Lemma typed_subst_typ s G t T :
+Lemma typed_closed G t T :
   typed G t T ->
+  typ_bv T = [::].
+Proof.
+  induction 1 => //=.
+  - apply /undup_nil /perm_eq_nilP /(uniq_perm_eq (undup_uniq _)) => // ?.
+    rewrite mem_undup. apply /negbTE /negP => /typ_bv_open [ ? [ ] ].
+    by rewrite H0.
+  - by rewrite H IHtyped.
+  - by move: IHtyped2 IHtyped1 => /= ->.
+Qed.
+
+Lemma typed_weaken G t T :
+  typed G t T ->
+  forall G',
+  (forall x, x < size G -> exists s, forall d d', nth d G x = typ_open s (nth d' G' x)) ->
+  typed G' t T.
+Proof.
+  induction 1 => /= G' HG'; eauto.
+  - case (leqP (size G) x) => [ ? | /HG' [ ? Hinst ] ].
+    { move: (H (typ_fvar 0)).
+      by rewrite -(H (typ_bvar 0)) !nth_default. }
+    rewrite -(H (typ_fvar 0)) (Hinst (typ_fvar 0) (typ_fvar 0)) typ_open_comp.
+    apply /typed_var => ?.
+    + apply /set_nth_default.
+      move: (leqP (size G') x) (Hinst (typ_fvar 0) (typ_fvar 0)) => [ ? | // ].
+      by rewrite (Hinst _ (typ_fvar 1)) !nth_default.
+    + apply /undup_nil /perm_eq_nilP /(uniq_perm_eq (undup_uniq _)) => // ?.
+      rewrite mem_undup.
+      apply /negbTE /negP => /typ_bv_open [ ? [ ] ].
+      by rewrite H0.
+  - apply /typed_abs => //.
+    apply /IHtyped => [ [ ? | ] /= ]; eauto.
+    exists typ_bvar. by rewrite typ_open_bvar.
+  - apply /typed_let; eauto.
+    apply /IHtyped => [ [ ? | ] /= ]; eauto.
+    exists typ_bvar. by rewrite typ_open_bvar.
+Qed.
+
+Lemma typed_subst_typ G t T :
+  typed G t T ->
+  forall s,
+  (forall x, typ_bv (s x) = [::]) ->
   typed (env_subst s G) t (typ_subst s T).
 Proof.
-  induction 1 => /=; eauto.
-  constructor => d.
-  case (leqP (size G) x) => ?.
-  - move: nth_default (H (typ_arrow T T))
-      => -> // /(f_equal typ_size) /= /eq_leq.
-    by rewrite ltnNge leq_addr.
-  - by rewrite (nth_map d) // H.
+  induction 1 => s0 Hclosed /=; eauto.
+  - rewrite typ_subst_open_distr => [ | ? ? ? ].
+    + apply /typed_var => ?.
+      * case (leqP (size G) x) => ?.
+         { move: (H (typ_fvar 0)).
+           by rewrite -(H (typ_bvar 0)) !nth_default // size_map. }
+         by rewrite /env_subst (nth_map (typ_fvar 0)) // H.
+      * apply /undup_nil /perm_eq_nilP /(uniq_perm_eq (undup_uniq _)) => // ?.
+        rewrite mem_undup.
+        { apply /negbTE /negP => /typ_bv_subst [ | [ ? [ ] ] ].
+          - by rewrite H0.
+          - by rewrite Hclosed. }
+    + by rewrite Hclosed.
+  - apply /typed_abs.
+    { apply /undup_nil /perm_eq_nilP /(uniq_perm_eq (undup_uniq _)) => // ?.
+      rewrite mem_undup. apply /negbTE /negP => /typ_bv_subst [ | [ ? [ ] ] ].
+      - by rewrite H.
+      - by rewrite Hclosed. }
+    exact /IHtyped.
+  - apply /(typed_let (env_fv G ++ typ_fv T1 ++ L)) => [ s' Hs' | ]; [ | exact /IHtyped ].
+    rewrite -(typ_subst_ext (fun x => if (x \notin env_fv G) && (x \notin typ_fv T1) then typ_fvar x else s0 x)) => [ | ? -> /= ].
+    + rewrite typ_open_subst_distr => [ | x ? ? ].
+      { rewrite -(typ_subst_ext (fun x => if (x \notin env_fv G) && (x \notin typ_fv T1) then typ_fvar x else s0 x)) => [ | /= ? /typ_fv_open [ -> /= | [ x [ ] ] ] ].
+        - rewrite -(env_subst_ext (fun x => if (x \notin env_fv G) && (x \notin typ_fv T1) then typ_fvar x else s0 x)) => [ | ? -> // ].
+          apply H0 => x.
+          + case (Hs' x) => ? [ -> ].
+            rewrite !mem_cat !negb_or => /andP [ ? /andP [ ] ]. eauto.
+          + by rewrite (fun_if typ_bv) /= Hclosed if_same.
+        - rewrite andbF typ_open_bvar_eq => // ?.
+          by rewrite Hclosed.
+        - case (Hs' x) => ? [ -> /= ].
+          rewrite mem_seq1 !mem_cat !negb_or => /andP [ HG /andP [ HT1 ? ] ] /eqP ?.
+          subst. by rewrite HG HT1. }
+      case (Hs' x) => ? [ -> /= ].
+      rewrite mem_seq1 !mem_cat !negb_or => /andP [ HG /andP [ HT1 ? ] ] /eqP ?.
+      subst. by rewrite HG HT1.
+    + by rewrite andbF.
 Qed.
 Hint Resolve typed_subst_typ.
 
-Definition gensym := succn \o foldr maxn 0.
+Definition maximum := foldr maxn 0.
 
-Lemma gensym_fresh L : gensym L \notin L.
+Lemma maximum_sup : forall xs x, x \in xs -> x <= maximum xs.
 Proof.
-  have IH : forall x, x \in L -> x < gensym L.
-  { elim L => //= ? ? IH ?.
-    rewrite in_cons => /orP [ /eqP <- | /IH ];
-    rewrite /gensym /= !ltnS leq_max ?leqnn // => ->.
-    by rewrite orbT. }
-  apply /negP => /IH.
-  by rewrite ltnn.
+  elim => //= ? ? IH ?.
+  rewrite in_cons => /orP [ /eqP <- | /IH ];
+  rewrite leq_max ?leqnn // => ->.
+  by rewrite orbT.
 Qed.
 
-Fixpoint typing L G t :=
+Fixpoint typing n G t :=
   match t with
-  | trm_var x => nth None (map (Some \o pair (L, typ_fvar)) G) x
-  | trm_abs t =>
-      let x := gensym L in
-      match typing (x :: L) (typ_fvar x :: G) t with
+  | trm_var x =>
+      match nth None (map Some G) x with
       | None => None
-      | Some (L, s, T2) => Some (L, s, typ_arrow (s x) T2)
+      | Some T => Some ((n + maximum (typ_bv T)).+1, typ_fvar, typ_open (typ_fvar \o addn n) T)
+      end
+  | trm_abs t =>
+      match typing n.+1 (typ_fvar n :: G) t with
+      | None => None
+      | Some (m, s, T2) => Some (m, s, typ_arrow (s n) T2)
       end
   | trm_app t1 t2 =>
-      match typing L G t1 with
+      match typing n G t1 with
       | None => None
-      | Some (L1, s1, T1) =>
-          match typing L1 (env_subst s1 G) t2 with
+      | Some (n1, s1, T1) =>
+          match typing n1 (env_subst s1 G) t2 with
           | None => None
-          | Some (L2, s2, T2) =>
-              let x := gensym L2 in
+          | Some (n2, s2, T2) =>
               option_map
-                (fun s3 => (x :: L2, typ_subst (typ_subst s3 \o s2) \o s1, s3 x))
-                (unify (typ_subst s2 T1) (typ_arrow T2 (typ_fvar x)))
+                (fun s3 => (n2.+1, typ_subst (typ_subst s3 \o s2) \o s1, s3 n2))
+                (unify (typ_subst s2 T1) (typ_arrow T2 (typ_fvar n2)))
           end
       end
   | trm_let t1 t2 =>
-      match typing L G t1 with
+      match typing n G t1 with
       | None => None
-      | Some (L1, s1, T1) =>
-          match typing L1 (T1 :: env_subst s1 G) t2 with
+      | Some (n1, s1, T1) =>
+          match typing n1 (typ_subst (fun x => if x \in env_fv (env_subst s1 G) then typ_fvar x else typ_bvar x) T1 :: env_subst s1 G) t2 with
           | None => None
-          | Some (L2, s2, T2) => Some (L2, typ_subst s2 \o s1, T2)
+          | Some (n2, s2, T2) => Some (n2, typ_subst s2 \o s1, T2)
           end
       end
   end.
 
-Theorem typing_sound : forall t L L' G s T,
-  typing L G t = Some (L', s, T) ->
-  typed (env_subst s G) t T.
+(* let f = fun x -> x in f f *)
+Eval compute in (typing 0 [::] (trm_let (trm_abs (trm_var 0)) (trm_app (trm_var 0) (trm_var 0)))).
+(* (fun f -> f f) (fun x -> x) *)
+Eval compute in (typing 0 [::] (trm_app (trm_abs (trm_app (trm_var 0) (trm_var 0))) (trm_abs (trm_var 0)))).
+
+Theorem typing_sound : forall t n m G s T,
+  typing n G t = Some (m, s, T) ->
+  typed (env_subst s G) t T /\ forall x, typ_bv (s x) = [::].
 Proof.
-  elim => /= [ x ? ? G ? ? Hnth | t IHt L ? G ? ? | t1 IHt1 t2 IHt2 L ? G ? ? | t1 IHt1 t2 IHt2 L ? G ? ? ].
-  - apply /typed_var => d.
-    move: (leqP (size G) x) Hnth => [ ? | /(nth_map d _) -> ].
+  elim => /=
+    [ x ? ? G ? ?
+    | t IHt n ? G ? ?
+    | t1 IHt1 t2 IHt2 n ? G ? ?
+    | t1 IHt1 t2 IHt2 n ? G ? ? ].
+  - case (leqP (size G) x) => ?.
     + by rewrite nth_default // size_map.
-    + inversion 1. by rewrite env_subst_typ_fvar.
-  - destruct (typing (gensym L :: L) (typ_fvar (gensym L) :: G) t) as [ [ [ ? ? ] ] | ] eqn:Htyping; inversion 1. subst.
-    exact /typed_abs /(IHt _ _ _ _ _ Htyping).
-  - destruct (typing L G t1) as [ [ [ L1 s1 ] T1 ] | ] eqn:Htyping1 => //.
-    destruct (typing L1 (env_subst s1 G) t2) as [ [ [ L2 s2 ] T2 ] | ] eqn:Htyping2 => //.
-    destruct (unify (typ_subst s2 T1) (typ_arrow T2 (typ_fvar (gensym L2)))) as [ s3 | ] eqn:Hunify; inversion 1. subst.
-    rewrite -!env_subst_typ_comp.
-    apply /(typed_app _ _ _ (typ_subst s3 T2)); eauto.
-    move: (unify_sound _ _ _ Hunify) => /= <-. eauto.
-  - destruct (typing L G t1) as [ [ [ L1 s1 ] T1 ] | ] eqn:Htyping1 => //.
-    destruct (typing L1 (T1 :: env_subst s1 G) t2) as [ [ [ ? s2 ] ? ] | ] eqn:Htyping2; inversion 1. subst.
-    rewrite -!env_subst_typ_comp.
-    apply /typed_let; eauto.
-    exact (IHt2 _ _ _ _ _ Htyping2).
+    + rewrite (nth_map (typ_fvar 0)) //. inversion 1.
+      rewrite env_subst_fvar.
+      split => [ | ? // ].
+      apply /typed_var => // ?.
+      exact /set_nth_default.
+  - destruct (typing n.+1 (typ_fvar n :: G) t) as [ [ [ ? ? ] ] | ] eqn:Htyping; inversion 1. subst.
+    move: (IHt _ _ _ _ _ Htyping) => [ ? ? ]. eauto.
+  - destruct (typing n G t1) as [ [ [ n1 s1 ] T1 ] | ] eqn:Htyping1 => //.
+    destruct (typing n1 (env_subst s1 G) t2) as [ [ [ n2 s2 ] T2 ] | ] eqn:Htyping2 => //.
+    destruct (unify (typ_subst s2 T1) (typ_arrow T2 (typ_fvar n2))) as [ s3 | ] eqn:Hunify; inversion 1. subst.
+    case (IHt1 _ _ _ _ _ Htyping1) => ? Hs1bv.
+    case (IHt2 _ _ _ _ _ Htyping2) => Htyped2 Hs2bv.
+    have Htyped1' : typed (env_subst s2 (env_subst s1 G)) t1 (typ_subst s2 T1); eauto.
+    have : forall x : nat, typ_bv (s3 x) = [::] => Hs3bv.
+    { apply /undup_nil /perm_eq_nilP /(uniq_perm_eq (undup_uniq _)) => // ?.
+      rewrite mem_undup.
+      apply /negbTE /negP => /(unify_bound _ _ _ Hunify) /orP /=.
+      by rewrite (typed_closed _ _ _ Htyped1') mem_cat (typed_closed _ _ _ Htyped2). }
+    split => [ | ? ].
+    + rewrite -!env_subst_comp.
+      apply /(typed_app _ _ _ (typ_subst s3 T2)).
+      * move: (unify_sound _ _ _ Hunify) => /= <-.
+        apply /typed_subst_typ; eauto.
+      * apply /typed_subst_typ; eauto.
+    + apply /undup_nil /perm_eq_nilP /(uniq_perm_eq (undup_uniq _)) => // ?.
+      rewrite mem_undup.
+      apply /negbTE /negP => /typ_bv_subst [ | [ ? [ /typ_bv_subst [ | [ ? [ ] ] ] ] ] ].
+      + by rewrite Hs1bv.
+      + by rewrite Hs2bv.
+      + by rewrite Hs3bv.
+  - destruct (typing n G t1) as [ [ [ n1 s1 ] T1 ] | ] eqn:Htyping1 => //.
+    destruct (typing n1 (typ_subst (fun x => if x \in env_fv (env_subst s1 G) then typ_fvar x else typ_bvar x) T1 :: env_subst s1 G) t2) as [ [ [ n2 s2 ] T2 ] | ] eqn:Htyping2;
+    rewrite Htyping2; inversion 1. subst.
+    case (IHt1 _ _ _ _ _ Htyping1) => Htyped1 Hclosed1.
+    case (IHt2 _ _ _ _ _ Htyping2) => ? Hclosed2.
+    split => [ | ? ].
+    + rewrite -env_subst_comp.
+      apply /(typed_let (env_fv (env_subst s1 G))) => [ s Hs | ]; eauto.
+      rewrite typ_subst_comp typ_open_subst_distr => [ | ? ].
+      { rewrite typ_open_bvar_eq => [ | ? ].
+        - rewrite (env_subst_ext s2 (typ_open s \o (typ_subst s2 \o (fun x => if x \in env_fv (env_subst s1 G) then typ_fvar x else typ_bvar x)))) => [ | ? /= -> /= ].
+          + apply /typed_subst_typ => //= x.
+            apply /undup_nil /perm_eq_nilP /(uniq_perm_eq (undup_uniq _)) => // ?.
+            rewrite mem_undup.
+            apply /negbTE /negP => /typ_bv_open [ y [ ] ].
+            case (Hs y) => ? [ -> // ].
+          + rewrite typ_open_bvar_eq => // ?.
+            by rewrite Hclosed2.
+        - by rewrite (typed_closed _ _ _ Htyped1). }
+      by rewrite (typed_closed _ _ _ Htyped1).
+    + apply /undup_nil /perm_eq_nilP /(uniq_perm_eq (undup_uniq _)) => // ?.
+      rewrite mem_undup.
+      apply /negbTE /negP => /typ_bv_subst [ | [ ? [ ] ] ].
+      * by rewrite Hclosed1.
+      * by rewrite Hclosed2.
 Qed.
 
-Theorem typing_complete : forall t L G s T,
-  { subset env_fv G <= L } ->
+Theorem typing_complete : forall t n G s T,
+  {in env_fv G, forall x, typ_bv (s x) = [::]} ->
+  (forall x, x \in env_fv G -> x < n) ->
   typed (env_subst s G) t T ->
-  exists L' s' s'' T', typing L G t = Some (L', s', T')
-    /\ { subset L <= L' } /\ T = typ_subst s'' T'
-    /\ (forall x y, x \in typ_fv (s' y) -> x = y \/ x \in L')
-    /\ { subset typ_fv T' <= L' }
-    /\ { in L, s =1 typ_subst s'' \o s' }.
+  exists m s' s'' T', typing n G t = Some (m, s', T')
+    /\ n <= m
+    /\ T = typ_subst s'' T'
+    /\ typ_bv T' = [::]
+    /\ (forall x, typ_bv (s' x) = [::])
+    /\ (forall x y, x \in typ_fv (s' y) -> x = y \/ x < m)
+    /\ (forall x, x \in typ_fv T' -> x < m)
+    /\ (forall x, x < n -> s x = typ_subst s'' (s' x)).
 Proof.
-  elim => /= [ x | t IHt | t1 IHt1 t2 IHt2 | t1 IHt1 t2 IHt2 ] L G s T HG; inversion 1; subst.
+  elim => /= [ x | t IHt | t1 IHt1 t2 IHt2 | t1 IHt1 t2 IHt2 ] n G s T Hclos HG; inversion 1; subst.
   - case (leqP (size G) x) => ?.
-    { move: (H2 (typ_fvar 0)).
-      by rewrite -(H2 (typ_bvar 0)) !nth_default // size_map. }
-    exists L, typ_fvar, s, (nth (typ_fvar 0) G x).
-    (repeat split) => [ | // | | ? ? /= | ? ? ].
+    { move: (H1 (typ_fvar 0)).
+      by rewrite -(H1 (typ_bvar 0)) !nth_default // size_map. }
+    exists ((n + maximum (typ_bv (nth (typ_fvar 0) G x))).+1), typ_fvar, (fun x => if x < n then s x else s0 (x - n)), (typ_open (typ_fvar \o addn n) (nth (typ_fvar 0) G x)).
+    (repeat split) => [ | | | | ? ? /= | ? /typ_fv_open [ ? | [ ? [ /= ] ] ] | ? /= -> // ].
     + by rewrite (nth_map (typ_fvar 0)).
-    + by rewrite -(H2 (typ_fvar 0)) /env_subst (nth_map (typ_fvar 0)).
+    + apply /leqW /leq_addr.
+    + rewrite -(H1 (typ_fvar 0)) /env_subst (nth_map (typ_fvar 0)) // typ_subst_open_distr => [ | /= x0 ? ? ].
+      { rewrite (typ_subst_ext (fun x => if x < n then s x else s0 (x - n)) s) => [ | ? ? ].
+        - apply /typ_open_ext => ? ? /=.
+          by rewrite ltnNge leq_addr /= addKn.
+        - by rewrite HG // (env_fv_intro (nth (typ_fvar 0) G x)) // mem_nth. }
+      by rewrite HG ?Hclos // (env_fv_intro (nth (typ_fvar 0) G x)) // mem_nth.
+    + apply /undup_nil /perm_eq_nilP /(uniq_perm_eq (undup_uniq _)) => // ?.
+      rewrite mem_undup. apply /negbTE /negP => /typ_bv_open [ ? [ //= ] ].
     + rewrite mem_seq1 => /eqP. eauto.
-    + apply /HG /env_fv_intro; eauto.
+    + apply /leqW /ltn_addr /HG /(env_fv_intro (nth (typ_fvar 0) G x)) => //.
       exact /mem_nth.
-  - move: (IHt (gensym L :: L) (typ_fvar (gensym L) :: G) (fun x => if x \in L then s x else T1) T2) => /= [ ? | | L' [ s' [ s'' [ T' [ -> [ HL' [ -> [ Hs' [ HT' Hgen ] ] ] ] ] ] ] ] ].
-    + rewrite !in_cons => /orP [ -> // | /HG -> ].
-      by rewrite orbT.
-    + by rewrite (negbTE (gensym_fresh _)) -(env_subst_ext s) => // ? /HG ->.
-    + exists L', s', s'', (typ_arrow (s' (gensym L)) T').
-      (repeat split) => [ ? ? | | // | ? /= | ? Hin ].
-      * apply /HL'. rewrite in_cons. apply /orP. eauto.
-      * move: (Hgen (gensym L)).
-        rewrite in_cons eqxx (negbTE (gensym_fresh _)) => -> //.
-      * rewrite mem_cat => /orP [ /Hs' [ ] -> | /HT' ] //.
-        apply /HL'. by rewrite in_cons eqxx.
-      * by rewrite -Hgen ?in_cons Hin // orbT.
-  - move: (IHt1 L G s (typ_arrow T1 T)) => [ ] // L1 [ s1 [ s' [ T2' [ -> [ HL1 [ HT [ Hs1fv [ HTfv Hs ] ] ] ] ] ] ] ].
-    move: (IHt2 L1 (env_subst s1 G) s' T1) => [ ? /env_fv_subst [ ? [ /Hs1fv [ -> /HG /HL1 | ] // ] ] | | L2 [ s2 [ s'' [ T1' [ -> [ HL2 [ HT1 [ Hs2fv [ HT1fv Hs' ] ] ] ] ] ] ] ] ].
-    { by rewrite env_subst_typ_comp -(env_subst_ext s) => // ? /HG /Hs. }
-    move: (unify_complete (typ_subst s2 T2') (typ_arrow T1' (typ_fvar (gensym L2))) (fun x => if x \in L2 then s'' x else T)) => [ | s3 [ -> [ [ s''' Hgen ] Hs3fv ] ] ] /=.
-    { rewrite (negbTE (gensym_fresh _)) !(typ_subst_ext (fun x => if x \in L2 then s'' x else T) s'') => [ | ? /HT1fv -> | ? /typ_fv_subst [ ? [ /Hs2fv [ <- /HTfv /HL2 | ] -> ] ] ] //.
+    + rewrite mem_seq1 => /eqP -> ?.
+      by rewrite ltnS leq_add2l maximum_sup.
+  - move: (IHt n.+1 (typ_fvar n :: G) (fun x => if x < n then s x else T1) T2) => /= [ x | ? | | n1 [ s1 [ s' [ T' [ -> [ Hn1 [ -> [ ? [ Hs1bv [ Hs1fv [ HT'fv Hs1 ] ] ] ] ] ] ] ] ] ] ].
+    { rewrite in_cons => /orP [ /eqP -> | Hin ].
+      - by rewrite ltnn H1.
+      - by rewrite HG // Hclos. }
+    { rewrite in_cons => /orP [ /eqP -> | /HG /leqW // ].
+      exact /leqnn. }
+    { by rewrite ltnn -(env_subst_ext s) => // ? /HG ->. }
+    exists n1, s1, s', (typ_arrow (s1 n) T').
+    (repeat split) => //= [ | | | ? | ? Hlt ].
+    + exact /ltnW.
+    + by rewrite -Hs1 // ltnn.
+    + by rewrite Hs1bv.
+    + by rewrite mem_cat => /orP [ /Hs1fv [ -> | ] | /HT'fv ].
+    + rewrite -Hs1 ?Hlt => //. exact /leqW.
+  - move: (IHt1 n G s (typ_arrow T1 T)) => [ ] // n1 [ s1 [ s' [ T2' [ -> [ Hn1 [ HT [ HT2'bv [ Hs1bv [ Hs1fv [ HTfv Hs ] ] ] ] ] ] ] ] ] ].
+    move: (IHt2 n1 (env_subst s1 G) s' T1) => [ ? /env_fv_subst [ x [ ? ? ] ] | ? /env_fv_subst [ ? [ /Hs1fv [ -> /HG /((@leq_trans _ _ _)^~Hn1) | ] // ] ] | | n2 [ s2 [ s'' [ T1' [ -> [ Hn2 [ HT1 [ HT1'bv [ Hs2bv [ Hs2fv [ HT1fv Hs' ] ] ] ] ] ] ] ] ] ] ].
+    { apply /undup_nil /perm_eq_nilP /(uniq_perm_eq (undup_uniq _)) => // z.
+      rewrite mem_undup.
+      apply /negbTE /negP => ?.
+      have : z \in typ_bv (typ_subst s' (s1 x)).
+      { apply /typ_bv_subst_intro_sub; eauto. }
+      by rewrite -Hs ?Hclos ?HG. }
+    { by rewrite env_subst_comp -(env_subst_ext s) => // ? /= /HG /Hs. }
+    move: (unify_complete (typ_subst s2 T2') (typ_arrow T1' (typ_fvar n2)) (fun x => if x < n2 then s'' x else T)) => [ | s3 [ Hunify [ [ s''' Hgen ] Hs3fv ] ] ] /=.
+    { rewrite ltnn !(typ_subst_ext (fun x => if x < n2 then s'' x else T) s'') => [ | ? /HT1fv -> | ? /typ_fv_subst [ ? [ /Hs2fv [ ] -> // /HTfv /((@leq_trans _ _ _)^~Hn2) -> ] ] ] //.
       rewrite typ_subst_comp (typ_subst_ext (typ_subst s'' \o s2) s') => [ | ? /HTfv /Hs' -> // ].
       congruence. }
-    exists (gensym L2 :: L2), (typ_subst (typ_subst s3 \o s2) \o s1), s''', (s3 (gensym L2)).
-    (repeat split) => [ ? /HL1 /HL2 | | ? ? /= | ? | ? ? /= ].
-    + rewrite in_cons => ->. by rewrite orbT.
-    + by rewrite -(Hgen (typ_fvar (gensym L2))) /= (negbTE (gensym_fresh _)).
-    + rewrite in_cons -!typ_subst_comp => /typ_fv_subst [ ? [ /Hs3fv /= [ <- /typ_fv_subst [ ? [ /Hs2fv [ <- /Hs1fv [ | /HL2 -> ] | -> ] ] ] | [ /typ_fv_subst [ ? [ /Hs2fv [ <- /HTfv /HL2 | ] -> ] ] | ] ] ] ];
-      rewrite ?orbT; eauto.
-      rewrite mem_cat mem_seq1 => /orP [ /HT1fv | ] ->; rewrite ?orbT; eauto.
-    + rewrite in_cons => /Hs3fv [ /eqP -> | /= [ /typ_fv_subst [ ? [ /Hs2fv [ <- /HTfv /HL2 -> | -> ] ] ] | ] ];
-      rewrite ?orbT // mem_cat mem_seq1 => /orP [ /HT1fv | ] -> //.
-      by rewrite orbT.
+    rewrite Hunify.
+    have : forall x, typ_bv (s3 x) = [::] => Hs3bv.
+    { apply /undup_nil /perm_eq_nilP /(uniq_perm_eq (undup_uniq _)) => // ?.
+      rewrite mem_undup.
+      apply /negbTE /negP => /(unify_bound _ _ _ Hunify) [ /typ_bv_subst [ | [ ? [ ] ] ] | /= ].
+      - by rewrite HT2'bv.
+      - by rewrite Hs2bv.
+      - by rewrite HT1'bv. }
+    exists n2.+1, (typ_subst (typ_subst s3 \o s2) \o s1), s''', (s3 n2).
+    (repeat split) => [ | | | x | ? ? /typ_fv_subst [ ? [ /typ_fv_subst [ ? [ /Hs3fv [ -> /Hs2fv [ -> /Hs1fv [ | /((@leq_trans _ _ _)^~Hn2) ] | ] | [ /typ_fv_subst [ ? [ /Hs2fv [ -> /HTfv /((@leq_trans _ _ _)^~Hn2) | ] ] ] | /= ] ] ] ] ] ] | ? /Hs3fv [ -> | [ /typ_fv_subst [ ? [ /Hs2fv [ -> /HTfv /((@leq_trans _ _ _)^~Hn2) | ] ] ] | /= ] ] | ? ? /= ]; eauto.
+    + apply /leqW /leq_trans; eauto.
+    + by rewrite -(Hgen (typ_fvar n2)) /= ltnn.
+    + apply /undup_nil /perm_eq_nilP /(uniq_perm_eq (undup_uniq _)) => // ?.
+      rewrite mem_undup.
+      apply /negbTE /negP => /typ_bv_subst [ | [ ? [ /typ_bv_subst [ | [ ? [ ] ] ] ] ] ].
+      * by rewrite Hs1bv.
+      * by rewrite Hs2bv.
+      * by rewrite Hs3bv.
+    + rewrite mem_cat mem_seq1 => /orP [ /HT1fv | /eqP -> ]; eauto.
+    + rewrite mem_cat mem_seq1 => /orP [ /HT1fv | /eqP -> ]; eauto.
     + rewrite Hs // (typ_subst_ext s' (typ_subst s'' \o s2)) => [ | ? /Hs1fv /= [ -> | /Hs' -> // ] ].
       * rewrite -!typ_subst_comp -Hgen.
-        apply /typ_subst_ext => ? /typ_fv_subst [ ? [ /Hs2fv [ <- /Hs1fv [ -> | /HL2 -> ] | -> ] // ] ].
-        by rewrite HL2 // HL1.
-      * exact /Hs' /HL1.
-  - move: (IHt1 L G s T1) => [ ] // L1 [ s1 [ s' [ T1' [ -> [ HL1 [ HT [ Hs1fv [ HTfv Hs ] ] ] ] ] ] ] ].
-    move: (IHt2 L1 (T1' :: env_subst s1 G) s' T) => /= [ ? | | L2 [ s2 [ s'' [ T2' [ -> [ HL2 [ HT2 [ Hs2fv [ HT2fv Hs2 ] ] ] ] ] ] ] ] ].
-    { by rewrite mem_cat => /orP [ /HTfv | /env_fv_subst [ ? [ /Hs1fv [ <- /HG /HL1 | ] ] ] ]. }
-    { by rewrite env_subst_typ_comp -HT -(env_subst_ext s) => // ? /HG /Hs ->. }
-    eexists L2, (typ_subst s2 \o s1), s'', T2'.
-    (repeat split) => [ ? /HL1 /HL2 | | ? ? /typ_fv_subst [ ? [ /Hs2fv [ <- /Hs1fv [ | /HL2 ] | ] ] ] | | ? ? ]; eauto.
-    rewrite Hs // (typ_subst_ext s' (typ_subst s'' \o s2)) ?typ_subst_comp => [ | ? /Hs1fv [ -> /= | /Hs2 ] ] //=.
-    by rewrite Hs2 // HL1.
+        apply /typ_subst_ext => ? /typ_fv_subst [ ? [ /Hs2fv [ <- /Hs1fv [ -> | /((@leq_trans _ _ _)^~Hn2) -> ] | -> ] // ] ].
+        by rewrite ((@leq_trans _ _ _)^~Hn2) // ((@leq_trans _ _ _)^~Hn1).
+      * exact /Hs' /((@leq_trans _ _ _)^~Hn1).
+  - move: (IHt1 n G s (typ_open (typ_fvar \o addn (maximum (typ_fv T1 ++ env_fv (env_subst s G) ++ L)).+1) T1)) => [ | | | n1' [ s1 [ s' [ T1' [ -> [ Hn1 [ HT [ HT1'bv [ Hs1bv [ Hs1fv [ HTfv Hs ] ] ] ] ] ] ] ] ] ] ] //.
+    { apply /H3 => x. repeat eexists.
+      have : (maximum (typ_fv T1 ++ env_fv (env_subst s G) ++ L)).+1 + x \notin typ_fv T1 ++ env_fv (env_subst s G) ++ L.
+      { apply /negP => /maximum_sup.
+        by rewrite addSn ltnNge leq_addr. }
+      by rewrite !mem_cat !negb_or => /andP [ ? /andP [ ] ]. }
+    move: (IHt2 n1' (typ_subst (fun x => if x \in env_fv (env_subst s1 G) then typ_fvar x else typ_bvar x) T1' :: env_subst s1 G) s' T) =>
+      /= [ ? | ? | | n2' [ s2 [ s'' [ T2' [ -> [ Hn2 [ HT2' [ HT2'bv [ Hs2bv [ Hs2fv [ HT2fv Hs' ] ] ] ] ] ] ] ] ] ] ] //.
+    { rewrite mem_cat => /orP [ /typ_fv_subst [ x [ ] ] | /env_fv_subst [ x [ ? ? ] ] ].
+      - destruct (x \in env_fv (env_subst s1 G)) eqn:Hfv; rewrite Hfv //= mem_seq1 => /eqP <- ?.
+        apply /undup_nil /perm_eq_nilP /(uniq_perm_eq (undup_uniq _)) => // z.
+        rewrite mem_undup.
+        apply /negbTE /negP => ?.
+        have : z \in typ_bv (typ_subst s' T1').
+        { apply /typ_bv_subst_intro_sub; eauto. }
+        by rewrite -HT => /typ_bv_open [ ? [ ] ].
+      - apply /undup_nil /perm_eq_nilP /(uniq_perm_eq (undup_uniq _)) => // z.
+        rewrite mem_undup.
+        apply /negbTE /negP => ?.
+        have : z \in typ_bv (typ_subst s' (s1 x)).
+        { apply/ typ_bv_subst_intro_sub; eauto. }
+        by rewrite -Hs ?Hclos ?HG. }
+    { rewrite mem_cat => /orP [ /typ_fv_subst [ y [ ] ] | /env_fv_subst [ ? [ /Hs1fv [ -> /HG /((@leq_trans _ _ _)^~Hn1) | ] ] ] ] //.
+      move: (y \in env_fv (env_subst s1 G)) => [ /= | // ].
+      by rewrite mem_seq1 => /eqP -> /HTfv. }
+    { apply /(typed_weaken _ _ _ H5) => [ [ ? | ? Hlt ] /= ].
+      - move: (f_equal (typ_subst (fun x => if x <= maximum (typ_fv T1 ++ env_fv (env_subst s G) ++ L) then typ_fvar x else typ_bvar (x - (maximum (typ_fv T1 ++ env_fv (env_subst s G) ++ L)).+1))) HT).
+        rewrite typ_subst_open_distr => [ | x Hin ? ].
+        + rewrite typ_subst_fvar_eq => [ | x Hin ].
+          { rewrite typ_open_bvar_eq => [ -> | ? ? /= ].
+            - exists (typ_subst (fun x => if x <= maximum (typ_fv T1 ++ env_fv (env_subst s G) ++ L) then typ_fvar x else typ_bvar (x - (maximum (typ_fv T1 ++ env_fv (env_subst s G) ++ L)).+1)) \o s') => ? ?.
+              rewrite !typ_subst_comp typ_open_subst_distr => [ | ? ].
+              + rewrite typ_open_bvar_eq => [ | ? ].
+                { apply /typ_subst_ext => x ? /=.
+                  rewrite fun_if /= fun_if /=.
+                  destruct (x \in env_fv (env_subst s1 G)) eqn:Henv; rewrite Henv //.
+                  rewrite typ_open_bvar_eq => [ | y ? ].
+                  - rewrite typ_subst_fvar_eq => [ // | y Hin ].
+                    rewrite maximum_sup // !mem_cat -(env_subst_ext (typ_subst s' \o s1)) => [ | ? /HG /Hs // ].
+                    by rewrite -env_subst_comp (env_fv_subst_intro _ _ x) // orbT.
+                  - have : y \in typ_bv (typ_subst s' T1').
+                    { apply /typ_bv_subst_intro_sub; eauto. }
+                    by rewrite -HT => /typ_bv_open [ ? [ ] ]. }
+                by rewrite HT1'bv.
+              + by rewrite HT1'bv.
+            - by rewrite addSn ltnNge leq_addr /= subSS addKn. }
+          by rewrite maximum_sup // mem_cat Hin.
+        + by rewrite maximum_sup // mem_cat Hin.
+      - exists typ_bvar => ? ?.
+        rewrite typ_open_bvar env_subst_comp (env_subst_ext (typ_subst s' \o s1) s) => [ | ? /HG /Hs // ].
+        apply /set_nth_default /Hlt. }
+    exists n2', (typ_subst s2 \o s1), s'', T2'.
+    (repeat split) => //= [ | ? | ? ? /typ_fv_subst [ ? [ /Hs2fv [ -> /Hs1fv [ | /((@leq_trans _ _ _)^~Hn2) ] | ] ] ] | ? ? ]; eauto.
+    + exact /(leq_trans Hn1).
+    + apply /undup_nil /perm_eq_nilP /(uniq_perm_eq (undup_uniq _)) => // ?.
+      rewrite mem_undup. apply /negbTE /negP => /typ_bv_subst [ | [ ? [ ] ] ].
+      * by rewrite Hs1bv.
+      * by rewrite Hs2bv.
+    + rewrite Hs // (typ_subst_ext s' (typ_subst s'' \o s2)) ?typ_subst_comp => /= [ // | ? /Hs1fv [ -> | ] ];
+      apply /Hs'; exact /((@leq_trans _ _ _)^~Hn1).
 Qed.
