TypeSafety.v
@@ -9,27 +9,49 @@ Lemma typed_rename G t T :
   typed G' (rename r t) T.
 Proof.
   induction 1 => /= ? ? Hnth; eauto.
-  - apply /typed_var => ?.
+  - apply /typed_var => // ?.
     by rewrite -Hnth H.
-  - by apply /typed_abs /IHtyped => ? [ | ? ] /=.
+  - apply /typed_abs; eauto.
+    by apply /IHtyped => ? [ | ? ] /=.
   - apply /typed_let; eauto.
-    by apply /IHtyped2 => ? [ | ? ] /=.
+    by apply /IHtyped => ? [ | ? ] /=.
 Qed.
 
 Lemma typed_subst G t T :
   typed G t T ->
   forall s G',
-  (forall x T, (forall d, nth d G x = T) -> typed G' (s x) T) ->
+  ( forall x T, (forall d, nth d G x = T) ->
+    exists (L : seq _), forall s',
+    (forall x, exists y, s' x = typ_fvar y /\ y \notin L) ->
+    typed G' (s x) (typ_open s' T) ) ->
   typed G' t.[s] T.
 Proof.
-  induction 1 => /= ? ? Hnth; eauto.
-  - apply /typed_abs /IHtyped => [ [ ? /(_ (typ_fvar 0)) /= -> | ? ? Hnth' ] /= ].
-    + exact /typed_var.
-    + exact /(typed_rename _ _ _ (Hnth _ _ Hnth')).
+  induction 1 => /= s0 G' Hnth; eauto.
+  - move: (Hnth _ _ H) => [ L Hs' ].
+    rewrite -(env_subst_fvar G') -(typ_subst_fvar T)
+    -(env_subst_ext (fun x => if x <= maximum (env_fv G' ++ typ_fv T ++ L) then typ_fvar x else s (x - maximum (env_fv G' ++ typ_fv T ++ L)).-1)) => [ | ? Hin ].
+    + rewrite -(typ_subst_ext (fun x => if x <= maximum (env_fv G' ++ typ_fv T ++ L) then typ_fvar x else s (x - maximum (env_fv G' ++ typ_fv T ++ L)).-1)) => [ | ? Hin ].
+      { rewrite -(typ_open_ext (typ_subst (fun x => if x <= maximum (env_fv G' ++ typ_fv T ++ L) then typ_fvar x else s (x - maximum (env_fv G' ++ typ_fv T ++ L)).-1) \o (typ_fvar \o addn (maximum (env_fv G' ++ typ_fv T ++ L)).+1))) => [ | ? /typ_bv_subst [ ? | [ ? [ ] ] ] /= ].
+        - rewrite -typ_subst_open_distr => [ | ? ? ? ].
+          + apply /typed_subst_typ => [ | ? ].
+            * apply Hs' => y. repeat eexists. apply /negP => Hin.
+              have : (maximum (env_fv G' ++ typ_fv T ++ L)).+1 + y <= (maximum (env_fv G' ++ typ_fv T ++ L)).
+              { apply /maximum_sup. by rewrite !mem_cat Hin !orbT. }
+              by rewrite addSn ltnNge leq_addr.
+            * by rewrite fun_if H0 /= if_same.
+          + by rewrite fun_if H0 /= if_same.
+        - by rewrite addSn ltnNge leq_addr /= subSKn addnC addnK.
+        - by rewrite fun_if H0 /= if_same. }
+      by rewrite maximum_sup // !mem_cat Hin !orbT.
+    + by rewrite maximum_sup // !mem_cat Hin.
+  - apply /typed_abs; eauto.
+    apply /IHtyped => [ [ ? /(_ (typ_fvar 0)) /= -> | ? ? /= /Hnth [ L ? ] ] ].
+    + exists [::] => ? Hs. apply /typed_var => //= x. by case (Hs x) => ? [ -> ].
+    + exists L => ? ?. apply /typed_rename; eauto.
   - apply /typed_let; eauto.
-    apply /IHtyped2 => [ [ ? /(_ (typ_fvar 0)) /= -> | ? ? Hnth' ] /= ].
-    + exact /typed_var.
-    + exact /(typed_rename _ _ _ (Hnth _ _ Hnth')).
+    apply /IHtyped => [ [ ? /(_ (typ_fvar 0)) /= -> | ? ? /= /Hnth [ L' ? ] ] ].
+    + exists L => ? Hs. apply /typed_var => //= x. by case (Hs x) => ? [ -> ].
+    + exists L' => ? ?. apply /typed_rename; eauto.
 Qed.
 
 Lemma subject_reduction t t' :
@@ -41,15 +63,20 @@ Proof.
   induction 1; inversion 1; subst; eauto.
   - inversion H4. subst.
     apply /typed_subst; eauto.
-    move => [ ? /(_ (typ_fvar 0)) <- // | /= ? ? ? ]; eauto.
+    move => [ ? /(_ (typ_fvar 0)) <- /= | /= ? ? ? ]; exists [::] => ? Hs.
+    + rewrite -(typ_open_ext typ_bvar) ?typ_open_bvar => // ?. by rewrite H7.
+    + apply /typed_var => // x. by case (Hs x) => ? [ -> ].
   - apply /typed_subst; eauto.
-    move => [ ? /(_ (typ_fvar 0)) <- // | /= ? ? ? ]; eauto.
+    move => [ ? /(_ (typ_fvar 0)) <- /= | /= ? ? ? ]; eauto.
+    exists [::] => ? Hs.
+    apply /typed_var => // x. by case (Hs x) => ? [ -> ].
 Qed.
 
 Lemma canonical_arrow v T1 T2 :
   value v ->
   typed nil v (typ_arrow T1 T2) ->
   exists t, v = trm_abs t.
+
 Proof. inversion 1; eauto. Qed.
 
 Lemma progress t : forall T,
@@ -57,9 +84,12 @@ Lemma progress t : forall T,
   value t \/ exists t', cbv t t'.
 Proof.
   induction t; inversion 1; subst; eauto.
-  - move: (H2 (typ_fvar 0)).
-    by rewrite -(H2 (typ_bvar 0)) !nth_default.
+  - move: (H1 (typ_fvar 0)).
+    by rewrite -(H1 (typ_bvar 0)) !nth_default.
   - move: (IHt1 _ H3) => [ /((canonical_arrow _ _ _)^~H3) [ ? -> ] | [ ? ? ] ]; eauto.
     move: (IHt2 _ H5) => [ ? | [ ? ? ] ]; eauto.
-  - move: (IHt _ H3) => [ ? | [ ? ? ] ]; eauto.
+  - case (IHt (typ_open (typ_fvar \o addn (maximum L).+1) T1)) => [ | ? | [ ] ]; eauto.
+    apply H3 => x. repeat eexists.
+    apply /negP => /maximum_sup.
+    by rewrite addSn ltnNge leq_addr.
 Qed.
